\documentclass[26pt, letterpaper]{article}
\usepackage{mathtools}
\usepackage[margin=0.5cm]{geometry}

\title{Quadratic Formula Derivation}
\begin{document}
\huge{
\textbf{\underline{Quadratic Formula Derivation}}\\


\bigskip
$y = ax^2  + bx + c$
\bigskip

Now complete the square:
\bigskip

$y = a \left(x^2 + \frac{b}{a}x \right) + c$
\bigskip

$y = a \left[ \left(x^2 + \frac{b}{a}x + \frac{b^2}{4a^2} \right ) - \frac{b^2}{4a^2} \right ] + c$
\bigskip

$y = a \left[ \left(x + \frac{b}{2a} \right)^2 - \frac{b^2}{4a^2} \right] + c$
\bigskip

$y = a \left(x + \frac{b}{2a} \right)^2 - \frac{b^2}{4a} + c$
\bigskip

Now multiply by 4a:
\bigskip
  
$y = a \left(x + \frac{b}{2a} \right)^2 - \frac{b^2}{4a} + c$
\bigskip

Now set y to zero and solve for x:
\bigskip

$a \left(x + \frac{b}{2a} \right)^2 - \frac{b^2}{4a} + c = 0$
\bigskip

$a \left(x + \frac{b}{2a} \right)^2 = \frac{b^2}{4a} + c$
\bigskip

Now multiply by 4a:
\bigskip

$4a^2 \left(x + \frac{b}{2a} \right)^2 = b^2 - 4ac$
\bigskip

$\left(x + \frac{b}{2a} \right)^2 = \frac{b^2 - 4ac}{4a^2}$
\bigskip

$x + \frac{b}{2a} = \pm \sqrt{\frac{b^2 - 4ac}{4a^2}}$
\bigskip

$x + \frac{b}{2a} = \pm \frac{\sqrt{b^2 - 4ac}}{2a}$
\bigskip

$x = \frac{-b}{2a} \pm \frac{\sqrt{b^2 - 4ac}}{2a} \Longrightarrow x = \frac{-b \pm \sqrt{b^2 - 4ac}}{2a}$  


}

\end{document}